clight/interpreter.h
@@ -37,11 +37,13 @@ struct memory_region {
 };
 
 struct bpf_state {
-  unsigned int state_pc;
+  int state_pc;
   int bpf_flag;
   unsigned long long regsmap[11];
   unsigned int mrs_num;
   struct memory_region *mrs;
+  int ins_len;
+  const unsigned long long * ins;
 };
 
-unsigned long long bpf_interpreter(struct bpf_state *, int, unsigned int,  const unsigned long long *);
+unsigned long long bpf_interpreter(struct bpf_state *, unsigned int);
