src/DxState.v
@@ -5,7 +5,7 @@ From compcert.lib Require Import Integers.
 From dx Require Import ResultMonad IR.
 From dx.Type Require Bool Nat.
 
-From bpf.src Require Import IdentDef CoqIntegers DxIntegers DxValues DxFlag DxRegs DxMemRegion.
+From bpf.src Require Import IdentDef CoqIntegers DxIntegers DxValues DxFlag DxRegs DxMemRegion DxList64.
 
 From Coq Require Import List ZArith.
 Import ListNotations.
@@ -16,6 +16,8 @@ Record state := mkst {
   regs_st : regmap;
   mrs_num : nat;  (**r number of memory regions, put it here to guarantee align *)
   bpf_mrs : MyMemRegionsType;
+  ins_len : sint32_t;
+  ins     : MyListType;
   bpf_m   : Memory.mem;
 }.
 
@@ -27,6 +29,8 @@ Definition init_state: state := {|
   regs_st := init_regmap;
   mrs_num := 0;
   bpf_mrs := default_memory_regions;
+  ins_len := Int.zero;
+  ins     := default_list;
   bpf_m   := init_mem;
  |}.
 
@@ -38,6 +42,8 @@ Definition upd_pc (p: sint32_t) (st:state): state := {|
   regs_st := regs_st st;
   mrs_num := mrs_num st;
   bpf_mrs := bpf_mrs st;
+  ins_len := ins_len st;
+  ins     := ins st;
   bpf_m   := bpf_m st;
 |}.
 
@@ -47,6 +53,8 @@ Definition upd_pc_incr (st:state): state := {|
   regs_st := regs_st st;
   mrs_num := mrs_num st;
   bpf_mrs := bpf_mrs st;
+  ins_len := ins_len st;
+  ins     := ins st;
   bpf_m   := bpf_m st;
 |}.
 
@@ -58,20 +66,12 @@ Definition upd_flag (f: bpf_flag) (st:state): state := {|
   regs_st := regs_st st;
   mrs_num := mrs_num st;
   bpf_mrs := bpf_mrs st;
+  ins_len := ins_len st;
+  ins     := ins st;
   bpf_m   := bpf_m st;
 |}.
 
 Definition eval_mem_num (st:state): nat := (mrs_num st). (**r uint32_t -> nat*)
-
-(*
-Definition upd_mem_num_incr (st:state): state := {|
-  pc_loc  := pc_loc st;
-  flag    := flag st;
-  mem_num := Int.add (mem_num st) Int.one;
-  regs_st := regs_st st;
-  bpf_mrs := bpf_mrs st;
-  bpf_m   := bpf_m st;
-|}.*)
 
 Definition eval_reg (r: reg) (st:state): val64_t :=
   eval_regmap r (regs_st st).
@@ -82,29 +82,13 @@ Definition upd_reg (r:reg) (v:val64_t) (st:state): state := {|
   regs_st := upd_regmap r v (regs_st st);
   mrs_num := mrs_num st;
   bpf_mrs := bpf_mrs st;
+  ins_len := ins_len st;
+  ins     := ins st;
   bpf_m   := bpf_m st;
 |}.
 
 Definition eval_mem_regions (st:state): MyMemRegionsType := bpf_mrs st.
-(*
-Definition add_mem_region (mr: memory_region) (st:state): state :={|
-  pc_loc  := pc_loc st;
-  flag    := flag st;
-  mem_num := Int.add (mem_num st) Int.one;
-  regs_st := regs_st st;
-  bpf_mrs := MyMemRegionsAdd mr (bpf_mrs st);
-  bpf_m   := bpf_m st;
-|}.
 
-Definition add_mem_region_ctx (mr: memory_region) (st:state): state :={|
-  pc_loc  := pc_loc st;
-  flag    := flag st;
-  mem_num := Int.one;
-  regs_st := regs_st st;
-  bpf_mrs := MyMemRegionsAdd mr (bpf_mrs st);
-  bpf_m   := bpf_m st;
-|}.
-*)
 Definition eval_mem (st: state):Mem.mem := bpf_m st.
 
 Definition upd_mem (m: Mem.mem) (st: state): state := {| (**r never be used I guess *)
@@ -113,6 +97,8 @@ Definition upd_mem (m: Mem.mem) (st: state): state := {| (**r never be used I gu
   regs_st := regs_st st;
   mrs_num := mrs_num st;
   bpf_mrs := bpf_mrs st;
+  ins_len := ins_len st;
+  ins     := ins st;
   bpf_m   := m;
 |}.
 
@@ -160,36 +146,8 @@ Definition store_mem_reg (chunk: memory_chunk) (ptr: valptr8_t) (v: val64_t) (st
   | _ => upd_flag BPF_ILLEGAL_MEM st
   end.
 
-(*
-Definition load_mem (chunk: memory_chunk) (ptr: valu32_t) (st: state) :=
-  match ptr with
-  | Vptr b ofs =>
-    match Mem.load chunk (bpf_m st) b (Ptrofs.unsigned ofs) with
-    | Some res => res
-    | None => val64_zero
-    end
-  | _ => val64_zero
-  end.
-
-Definition store_mem_imm (chunk: memory_chunk) (ptr: valu32_t) (v: vals32_t) (st: state): state :=
-  match ptr with
-  | Vptr b ofs =>
-    match Mem.store chunk (bpf_m st) b (Ptrofs.unsigned ofs) v with
-    | Some m => upd_mem m st
-    | None => upd_flag BPF_ILLEGAL_MEM st
-    end
-  | _ => upd_flag BPF_ILLEGAL_MEM st
-  end.
-
-Definition store_mem_reg (chunk: memory_chunk) (ptr: valu32_t) (v: val64_t) (st: state): state :=
-  match ptr with
-  | Vptr b ofs =>
-    match Mem.store chunk (bpf_m st) b (Ptrofs.unsigned ofs) v with
-    | Some m => upd_mem m st
-    | None => upd_flag BPF_ILLEGAL_MEM st
-    end
-  | _ => upd_flag BPF_ILLEGAL_MEM st
-  end. *)
+Definition eval_ins_len (st: state): sint32_t := (ins_len st).
+Definition eval_ins (idx: sint32_t) (st: state): int64_t := MyListIndexs32 (ins st) idx.
 
 (******************** Dx Related *******************)
 
@@ -203,7 +161,7 @@ Definition store_mem_reg (chunk: memory_chunk) (ptr: valu32_t) (v: val64_t) (st:
 Definition state_struct_type: Ctypes.type := Ctypes.Tstruct state_id Ctypes.noattr.
 
 Definition state_struct_def: Ctypes.composite_definition := 
-  Ctypes.Composite state_id Ctypes.Struct [(pc_id, C_U32); (flag_id, C_S32); (regmaps_id, C_regmap); (mem_regs_id, mem_region_type); (mem_num_id, C_U32)] Ctypes.noattr.
+  Ctypes.Composite state_id Ctypes.Struct [(pc_id, C_S32); (flag_id, C_S32); (regmaps_id, C_regmap); (mem_regs_id, mem_region_type); (mem_num_id, C_U32); (ins_len_id, C_S32); (ins_id, C_U64_pointer)] Ctypes.noattr.
 
 Definition stateCompilableType := MkCompilableType state state_struct_type.
 
