proof/correctproof/correct_eval_pc.v
@@ -28,13 +28,12 @@ Section Eval_pc.
   Definition f : arrow_type args (M res) := DxMonad.eval_pc.
 
   Variable state_block: block. (**r a block storing all rbpf state information? *)
-  Variable ins_block: block.
 
   (* [fn] is the Cligth function which has the same behaviour as [f] *)
   Definition fn: Clight.function := f_eval_pc.
 
   Definition stateM_correct (st:unit) (v: val) (stm:stateM) (m: Memory.Mem.mem) :=
-    v = Vptr state_block Ptrofs.zero /\ match_state state_block ins_block stm m.
+    v = Vptr state_block Ptrofs.zero /\ match_state state_block stm m.
 
   (* [match_arg] relates the Coq arguments and the C arguments *)
   Definition match_arg_list : DList.t (fun x => x -> val -> stateM -> Memory.Mem.mem -> Prop) ((unit:Type) ::args) :=
